

$$1 \ a) \begin{vmatrix} i & j & k \\ 1 & 3 & 1 \\ 2 & -1 & 5 \end{vmatrix} = i \begin{vmatrix} 3 & 1 \\ -1 & 5 \end{vmatrix} - j \begin{vmatrix} 1 & 1 \\ 2 & 5 \end{vmatrix} + k \begin{vmatrix} 1 & 3 \\ 2 & -1 \end{vmatrix} = 16i - 3j - 7k$$

$$b) (i+2j) \times (2i-3j)$$

$$= \begin{vmatrix} i & j & k \\ 1 & 2 & 0 \\ 2 & -3 & 0 \end{vmatrix} = k \begin{vmatrix} 1 & 2 \\ 2 & -3 \end{vmatrix} + 0 + 0 = 0i + 0j - 7k$$

$$2) \begin{vmatrix} i & j & k \\ 2 & -1 & 5 \\ 1 & 3 & 1 \end{vmatrix} = i \begin{vmatrix} -1 & 5 \\ 3 & 1 \end{vmatrix} - j \begin{vmatrix} 2 & 5 \\ 1 & 1 \end{vmatrix} + k \begin{vmatrix} 2 & -1 \\ 1 & 3 \end{vmatrix} = -14i - 3j + 7k$$

$$\Rightarrow \sqrt{14^2 + 3^2 + 7^2} = \sqrt{230}$$

3/4